\documentclass{article}
% \usepackage{ctex}

\title{FORMULA}
% \author{张汉杰}
\author{Vainjoker}
\date{\today}

\begin{document}
    \maketitle
    \newpage
    
    $U(R)=Ri(t)$

    $U_c(t)=\frac{1}{c}\int^t_{-\infty}(\tau)d\tau$

    $i_{c}(t)=C\frac{dU_{c}(t)}{dt}$

    $i_{L}(t)=\frac{1}{L}\int _{-\infty}^{t}U_{L}(\tau)d\tau$

    $U_{L}(t)=L\frac{di_{L}(t)}{dt}$

    $K*f(t)=K[S(f(t))]$

    $f(t)*\delta(t)=f(t)$

    $f(t)*\delta'(t)=f'(t)*\delta^(-1)(t)=f^{-1}(t)*\delta(t)=f^{-1}(t)$

    $f(t)*\epsilon(t)=f(t)*\delta^{-1}(t)=f^{-1}(t)*\delta(t)=f^{-1}(t)$

    $\epsilon(t)*\epsilon(t)=t\epsilon(t)$

    $e^{-at}\epsilon(t)*e^{-at}\epsilon(t)=te^{-at}\epsilon(t)$

    $e{-a_1t}\epsilon(t)*e^{a_2t}\epsilon(t)=(e^{-a_1t}-e^{-a_2t})(\epsilon(t))/(a_2-a_1)$


\end{document}
